Full parser works too

Test/modules/parser.dfy
@@ -7,25 +7,25 @@ module NativeTypes {
 }
 abstract module NativePackedInt {
   import opened NativeTypes
-  //type Integer
-  function unpack(s: seq<byte>) : bool
+  type Integer
+  function unpack(s: seq<byte>) : Integer
 }
 
-//module NativePackedUint32 refines NativePackedInt {
-//  type Integer = int
-//}
+module NativePackedUint32 refines NativePackedInt {
+  type Integer = int
+}
 
 // Marshalling
 abstract module Marshalling {
   import opened NativeTypes
-  //type UnmarshalledType
-  //function parse(data: seq<byte>) : bool
+  type UnmarshalledType
+  function parse(data: seq<byte>) : UnmarshalledType
 }
 
 // Integer marshalling
 module IntegerMarshalling(Int: NativePackedInt) refines Marshalling {
-  //type UnmarshalledType = Int.Integer
-  function parse(data: seq<byte>) : bool
+  type UnmarshalledType = Int.Integer
+  function parse(data: seq<byte>) : UnmarshalledType
   {
     Int.unpack(data)
   }
@@ -33,21 +33,21 @@ module IntegerMarshalling(Int: NativePackedInt) refines Marshalling {
 
 
 // Sequence marshalling
-//abstract module SeqMarshalling(ElementMarshalling: Marshalling) refines Marshalling {
-//  type Element = ElementMarshalling.UnmarshalledType
-//  type UnmarshalledType = seq<Element>
-//}
-//abstract module UniformSizedElementSeqMarshallingCommon(elementMarshalling: Marshalling) refines SeqMarshalling(elementMarshalling) {
-//  function parse_prefix(data: seq<byte>) : (result: UnmarshalledType)
-//    ensures result == [ elementMarshalling.parse(data) ]
-//}
-//module IntegerSeqMarshalling(Int: NativePackedInt) refines UniformSizedElementSeqMarshallingCommon(IntegerMarshalling(Int)) {
-//}
+abstract module SeqMarshalling(ElementMarshalling: Marshalling) refines Marshalling {
+  type Element = ElementMarshalling.UnmarshalledType
+  type UnmarshalledType = seq<Element>
+}
+abstract module UniformSizedElementSeqMarshallingCommon(elementMarshalling: Marshalling) refines SeqMarshalling(elementMarshalling) {
+  function parse_prefix(data: seq<byte>) : (result: UnmarshalledType)
+    ensures result == [ elementMarshalling.parse(data) ]
+}
+module IntegerSeqMarshalling(Int: NativePackedInt) refines UniformSizedElementSeqMarshallingCommon(IntegerMarshalling(Int)) {
+}
 
 // Works
-//module Uint32SeqMarshalling { //refines IntegerSeqMarshalling(NativePackedUint32) {
-//  import X = IntegerSeqMarshalling(NativePackedUint32)
-//}
+module Uint32SeqMarshalling { //refines IntegerSeqMarshalling(NativePackedUint32) {
+  import X = IntegerSeqMarshalling(NativePackedUint32)
+}
 
 // Creates a type mismatch, presumably due to _Compile issues
 //module Uint32SeqMarshalling2 refines IntegerSeqMarshalling(NativePackedUint32) {
